Making the Array library compile. Removing some admitted in Double.

lib/Array.v
@@ -16,11 +16,12 @@ Parameter array : Type -> Type.
 
 Parameter length : forall T, array T -> nat.
 
-Parameter bagCard : forall T, BagCard (array T).
-Instance _bagCard : forall T, BagCard (array T) := bagCard. (* FIXME: Some mechanism to avoid this repeation? *)
+Instance bagCard T : BagCard (array T) := {|
+    card := @length T
+  |}.
 
 Parameter bagReadOption : forall T, BagReadOption nat T (array T).
-Instance _bagReadOption : forall T, BagReadOption nat T (array T) := bagReadOption.
+Instance _bagReadOption : forall T, BagReadOption nat T (array T) := bagReadOption. (* FIXME: Some mechanism to avoid this repeation? *)
 Instance bagRead T `{Inhab T} : BagRead nat T (array T) :=
   ReadOptionToRead nat T (array T).
 
@@ -110,22 +111,38 @@ Module ArrayList <: ArraySpec.
 
 Definition array := list.
 
-Definition length T := length : array T -> nat.
+Definition length : forall T, array T -> nat := length.
 
-Definition read_option T (a : array T) n := nth_option n a.
-Definition read T `{Inhab T} (a : array T) n := nth n a.
-Definition write T (a : array T) n t := update n t a : array T.
+Instance bagCard T : BagCard (array T) := {|
+    card := @length T
+  |}.
+
+Instance bagReadOption T : BagReadOption nat T (array T) := {|
+    read_option a n := nth_option n a
+  |}.
+Instance _bagReadOption : forall T, BagReadOption nat T (array T) := bagReadOption.
+Instance bagRead T `{Inhab T} : BagRead nat T (array T) :=
+  ReadOptionToRead nat T (array T).
+
+Instance bagUpdate T : BagUpdate nat T (array T) := {|
+    LibContainer.update a n t := update n t a
+  |}.
+Instance _bagUpdate : forall T, BagUpdate nat T (array T) := bagUpdate.
+Definition write {T} : array T -> nat -> T -> array T :=
+  LibContainer.update.
 
 Definition from_list T := id : list T -> array T.
 Definition to_list T := id : array T -> list T.
 
-Definition empty T := from_list nil : array T.
-Arguments empty [T].
+Instance bagEmpty T : BagEmpty (array T) := {|
+   empty := from_list nil
+ |}.
+Instance _bagEmpty : forall T, BagEmpty (array T) := bagEmpty.
 
-Lemma read_option_Some : forall T `{Inhab T} a n,
+Lemma read_option_Some : forall T `{Inhab T} (a : array T) n,
   n < length a ->
   read_option a n = Some (read a n).
-Proof. introv I. apply~ nth_option_Some. Qed.
+Proof. introv I. simpl. erewrite~ @nth_option_Some. Qed.
 
 Lemma read_option_None : forall T (a : array T) n,
   n >= length a ->
@@ -143,24 +160,28 @@ Lemma read_option_write_neq : forall T a (t : T) n1 n2,
   read_option (write a n1 t) n2 = read_option a n2.
 Proof.
   introv I D. tests I': (n1 < length a).
-   apply~ nth_option_update_neq.
-   unfolds write. rewrite~ update_out. unfolds length. nat_math.
+  - apply~ nth_option_update_neq.
+  - fequals. unfold write. apply~ update_out. unfolds length. nat_math.
 Qed.
 
 Lemma read_write_eq : forall T `{Inhab T} a (t : T) n,
   n < length a ->
   read (write a n t) n = t.
-Proof. introv I. apply nth_update_eq. unfolds length. nat_math. Qed.
+Proof. introv I. unfold write. simpl. rewrite~ nth_option_update_eq. Qed.
 
 Lemma read_write_neq : forall T `{Inhab T} a (t : T) n1 n2,
   n2 < length a ->
   n1 <> n2 ->
   read (write a n1 t) n2 = read a n2.
-Proof. introv I D. applys nth_update_neq D. unfolds length. nat_math. Qed.
+Proof.
+  introv I D. unfold write. simpl. tests I': (n1 < length a).
+  - rewrite~ nth_option_update_neq.
+  - rewrite~ update_ge_length. unfolds length. nat_math.
+Qed.
 
 Lemma write_length : forall T a (t : T) n,
   length (write a n t) = length a.
-Proof. introv. apply length_update. Qed.
+Proof. introv. apply~ length_update. Qed.
 
 Lemma from_list_length : forall T (l : list T),
   length (from_list l) = LibList.length l.
@@ -171,7 +192,7 @@ Lemma to_list_length : forall T (a : array T),
 Proof. reflexivity. Qed.
 
 Lemma empty_length : forall T,
-  length (@empty T) = 0.
+  length (empty : array T) = 0.
 Proof. reflexivity. Qed.
 
 Lemma from_list_read_option : forall T (l : list T) n,
@@ -184,29 +205,41 @@ Proof. reflexivity. Qed.
 
 Lemma from_list_read : forall T `{Inhab T} (l : list T) n,
   read (from_list l) n = nth n l.
-Proof. reflexivity. Qed.
+Proof.
+  introv. simpl. destruct nth_option eqn: E.
+  - forwards*: nth_option_defined E.
+  - symmetry. apply nth_option_length in E.
+    forwards A: nth_default_gt_length; [ apply~ E | apply~ A ].
+Qed.
 
 Lemma to_list_read : forall T `{Inhab T} (a : array T) n,
   nth n (to_list a) = read a n.
-Proof. reflexivity. Qed.
+Proof. introv. symmetry. apply~ from_list_read. Qed.
 
 End ArrayList.
 
 
 Module ArrayListExtra <: ArrayExtra (ArrayList).
 
-Export ArrayList.
+Include ArrayList.
 
 Definition map : forall T1 T2, (T1 -> T2) -> array T1 -> array T2 := LibList.map.
 
 Lemma map_length : forall T1 T2 (f : T1 -> T2) a,
   length (map f a) = length a.
-Proof. introv. apply length_map. Qed.
+Proof. introv. apply~ length_map. Qed.
 
 Lemma map_read : forall T1 T2 `{Inhab T1} `{Inhab T2} (f : T1 -> T2) a n,
   n < length a ->
   read (map f a) n = f (read a n).
-Proof. introv I. apply~ map_nth. Qed.
+Proof.
+  introv I. simpl. destruct nth_option eqn:E1.
+  - forwards E1': nth_option_defined E1. destruct (nth_option n a) eqn:E2.
+    + forwards E2': nth_option_defined E2. substs~. apply~ map_nth.
+    + apply nth_option_length in E2. erewrite <- map_length in E2.
+      apply nth_option_length in E2. rewrite E1 in E2. false~ E2.
+  - apply nth_option_length in E1. erewrite map_length in E1. false. nat_math.
+Qed.
 
 End ArrayListExtra.
 
